Uniqueness, Soundness, Completeness

SigmaAlgebra.v
@@ -2,6 +2,7 @@ Require Import Coq.Vectors.Vector.
 Require Import Coq.Classes.RelationClasses.
 Require Import Coq.Logic.Eqdep_dec.
 Require Import Coq.Arith.PeanoNat.
+Require Import Coq.Arith.Wf_nat.
 
 Require Import VectorQuantification.
 Require Import DependentFixpoint.
@@ -268,7 +269,121 @@ Module Type Algebraic(Import SigSpec: SignatureSpec).
       + trivial.
       + split;
           [ apply g_compat; exact (proj1 args_eq) | apply IH; exact (proj2 args_eq) ].
-  Qed.     
+  Qed.
+
+  Inductive FixF (s : Sort EmptySet): Type :=
+  | mkFixF : forall (op: Operation)
+               (subst: Var -> Sort EmptySet)
+               (wf_subst: WellFormed subst)
+               (args: FixF_args s subst _ (domain op))
+               (subsort: subsorts (applySubst subst (range op)) s), FixF s        
+  with
+  FixF_args (s: Sort EmptySet): forall (S : Var -> Sort EmptySet) (n : nat) (argSorts: t (Sort Var) n), Type :=
+  | FixF_args_nil : forall S, FixF_args s S 0 (nil _)
+  | FixF_args_cons : forall S n argSort argSorts,
+      FixF (applySubst S argSort) -> FixF_args s S n argSorts -> FixF_args s S _ (cons _ argSort _ argSorts).
+
+  Definition FixF_args_case0 s S
+             (P : forall S n (argSorts: t (Sort Var) n), FixF_args s S n argSorts -> Type)
+             (argSorts: t (Sort Var) 0)
+             (args: FixF_args s S 0 argSorts): P S 0 (nil _) (FixF_args_nil s S) -> P S 0 argSorts args :=
+    (fun n argSorts (args: FixF_args s S n argSorts) =>
+       match args as args' in FixF_args _ S' n argSorts'
+             return n = 0 -> P S' 0 (nil _) (FixF_args_nil s S') -> P S' n argSorts' args' with
+       | FixF_args_nil _ _ => fun _ r => r
+       | FixF_args_cons _ _ _ _ _ _ _ =>
+         fun eq _ => False_rect _ (@eq_rect_r nat 0 (fun n => match n with | 0 => True | _ => False end) I _ eq)
+       end) 0 argSorts args eq_refl.
+
+  Definition FixF_args_caseS' s S n
+             (argSorts: t (Sort Var) (Datatypes.S n))
+             (args: FixF_args s S (Datatypes.S n) argSorts):
+    forall (P : forall S (argSorts: t (Sort Var) (Datatypes.S n)), FixF_args s S (Datatypes.S n) argSorts -> Type),
+      (forall S argSort argSorts' arg args',
+          P S (cons _ argSort _ argSorts') (FixF_args_cons s S n argSort argSorts' arg args')) ->
+      P S argSorts args :=
+    match args with
+    | FixF_args_nil _ _ => fun devil => False_rect (@IDProp) devil
+    | FixF_args_cons _ _ _ _ _ hd tl => fun P H => H _ _ _ hd tl
+    end.
+    
+  Fixpoint FixF_args_to_F_args
+           (s: Sort EmptySet) (S: Var -> Sort EmptySet) (n: nat) (argSorts: t (Sort Var) n)
+           (args: FixF_args s S n argSorts) {struct args}: F_args FixF S argSorts :=
+    match args with
+    | FixF_args_nil _ _ => tt
+    | FixF_args_cons _ _ n argSort argSorts hd tl => (hd, FixF_args_to_F_args s _ n argSorts tl)
+    end.
+
+  Fixpoint F_args_to_FixF_args
+           (s: Sort EmptySet) (S: Var -> Sort EmptySet) (n: nat) (argSorts: t (Sort Var) n)
+           (args: F_args FixF S argSorts) {struct argSorts}: FixF_args s S n argSorts :=
+    match argSorts as argSorts' return F_args FixF S argSorts' -> FixF_args s S _ argSorts' with
+    | nil _ => fun _ => FixF_args_nil s S
+    | cons _ x _ xs => fun args => FixF_args_cons _ _ _ _ _ (fst args) (F_args_to_FixF_args s _ _ xs (snd args))
+    end args.
+  
+  Definition FixF_alg: forall s, F FixF s -> FixF s :=
+    fun s f => mkFixF s (op _ _ f) (subst _ _ f) (wf_subst _ _ f)
+                   (F_args_to_FixF_args _ _ _ _ (args _ _ f)) (subsort _ _ f).
+
+  Definition FixF_coalg: forall s, FixF s -> F FixF s :=
+    fun s f =>
+      match f with
+      | mkFixF _ op subst wf_subst args subsort =>
+        mkF _ _ op subst wf_subst (FixF_args_to_F_args _ _ _ _ args) subsort
+      end.
+  
+  Lemma FixF_alg_coalg: forall s f, FixF_coalg s (FixF_alg s f) = f.
+  Proof.
+    intros s f.
+    destruct f as [ op subst wf_subst args subsort ].
+    simpl.
+    assert (args_eq: forall s S n argSorts args,
+               FixF_args_to_F_args s S n argSorts (F_args_to_FixF_args s S n argSorts args) = args).
+    { clear ...
+      intros s S n argSorts.
+      induction argSorts as [ | argSort n argSorts IH ].
+      - intro args.
+        destruct args; reflexivity.
+      - intro args.
+        destruct args as [ arg args ].
+        simpl.
+        rewrite (IH args).
+        reflexivity. }
+    rewrite args_eq.
+    reflexivity.
+  Qed.
+
+  Lemma FixF_coalg_alg: forall s c, FixF_alg s (FixF_coalg s c) = c.
+  Proof.
+    intros s c.
+    destruct c as [ op subst wf_subst args subsort ].
+    unfold FixF_alg.
+    simpl.
+    assert (args_eq: forall s S n argSorts args,
+               F_args_to_FixF_args s S n argSorts (FixF_args_to_F_args s S n argSorts args) = args).
+    { clear ...
+      intros s S n argSorts args.
+      induction args as [ | ? ? ? ? ? ? ? IH ].
+      - reflexivity.
+      - simpl.
+        rewrite IH.
+        reflexivity. }        
+    rewrite args_eq.
+    reflexivity.
+  Qed.
+
+ 
+  Fixpoint FixF_size s (f: FixF s): nat :=
+    match f with
+    | mkFixF _ _ _ _ args _ =>
+      1 + ((fix FixF_args_size s S n argSorts (args : FixF_args s S n argSorts): nat :=
+              match args with
+              | FixF_args_nil _ _ => 0
+              | FixF_args_cons _ _ _ _ _ arg args => (FixF_size _ arg) + (FixF_args_size _ _ _ _ args)
+              end) _ _ _ _ args)
+    end.
     
   Section AlgebraFixpoint.
     Variable C: Sort EmptySet -> Type.
@@ -401,6 +516,9 @@ Module Type Algebraic(Import SigSpec: SignatureSpec).
           rewrite (IH (snd args) (proj2 dec)).
           reflexivity.
     Qed.
+
+    
+      
     
     Section HomomorphismModulo.
       Variable alg': SigmaAlgebra C.
@@ -532,10 +650,639 @@ Module Type Algebraic(Import SigSpec: SignatureSpec).
               { exact (IH (snd args) (proj2 accs)). }
       Qed.
       
+      Inductive AlgebraicallyGenerated: forall s, C' s -> Prop :=
+      | FromF : forall s op S WF_S args subsort,
+          GeneratedArgs (arity op) (domain op) S args ->
+          AlgebraicallyGenerated s (alg s (mkF C' s op S WF_S args subsort))
+      with GeneratedArgs: forall n (dom : t (Sort Var) n) S, F_args C' S dom -> Prop :=
+           | GeneratedArgs_nil: forall S, GeneratedArgs 0 (nil _) S tt
+           | GeneratedArgs_cons:
+               forall n s dom' S arg args,
+                 AlgebraicallyGenerated (applySubst S s) arg ->
+                 GeneratedArgs n dom' S args ->
+                 GeneratedArgs _ (cons _ s n dom') S (arg, args).
+
+      Fixpoint GeneratedArgs_nth n dom S args k (args_gen: GeneratedArgs n dom S args):
+        AlgebraicallyGenerated (applySubst S (nth dom k)) (F_args_nth _ S dom args k).
+      Proof.
+        revert k.
+        case args_gen.
+        - intros S' k; inversion k.
+        - intros n' s dom' S' arg args' arg_gen args_gen' k.
+          apply (Fin.caseS' k).
+          + exact arg_gen.
+          + intro k'.
+            exact (GeneratedArgs_nth n' dom' S' args' k' args_gen').
+      Defined.
+      
+      Fixpoint AlgebraicallyGenerated_ind'
+               (P : forall s c, AlgebraicallyGenerated s c -> Prop)
+               (case_nth:
+                  forall (s: Sort EmptySet) op (S: Var -> Sort EmptySet) (WF_S: WellFormed S)
+                    args (subsort: subsorts (applySubst S (range op)) s)
+                    (args_gen : GeneratedArgs (arity op) (domain op) S args),
+                    (forall k, P _ (F_args_nth _ S _ args k) (GeneratedArgs_nth _ _ S args k args_gen)) ->
+                    P s _ (FromF s op S WF_S args subsort args_gen)
+               )
+               s c gen {struct gen}: P s c gen.
+      Proof.
+        case gen as [ s op S WF_S args subsort args_gen ].
+        apply case_nth.
+        intro k.
+        apply
+          ((fix rec_args S n dom args args_gen :
+              forall (k: Fin.t n), P (applySubst S (nth dom k))
+                                (F_args_nth C' S dom args k)
+                                (GeneratedArgs_nth n  dom S args k args_gen) :=
+              match args_gen as args_gen' in GeneratedArgs n' dom' S' args' return
+                    forall (k: Fin.t n'), P (applySubst S' (nth dom' k))
+                                       (F_args_nth C' S' dom' args' k)
+                                       (GeneratedArgs_nth n' dom' S' args' k args_gen')
+              with
+              | GeneratedArgs_nil _ => Fin.case0 _
+              | GeneratedArgs_cons n s dom subst arg args arg_gen args_gen =>
+                fun (k: Fin.t (Datatypes.S n)) =>
+                  Fin.caseS' k (fun k => P (applySubst subst (nth (cons _ s n dom) k))
+                                        (F_args_nth C' subst (cons _ s n dom) (arg, args) k)
+                                        (GeneratedArgs_nth (Datatypes.S n) (cons _ s n dom) subst (arg, args) k
+                                                           (GeneratedArgs_cons n s dom subst arg args arg_gen args_gen)))
+                             (AlgebraicallyGenerated_ind' P case_nth _ _ arg_gen)
+                             (fun k => rec_args subst n dom args args_gen k)
+              end) S (arity op) (domain op) args args_gen k).
+      Qed.
+
+      Definition GeneratedArgs_hd n s dom S args (args_gen: GeneratedArgs (Datatypes.S n) (cons _ s n dom) S args):
+        AlgebraicallyGenerated (applySubst S s) (fst args) :=
+        GeneratedArgs_nth (Datatypes.S n) (cons _ s n dom) S args Fin.F1 args_gen.
+
+      Definition GeneratedArgs_caseS n dom S args (args_gen: GeneratedArgs (Datatypes.S n) dom S args):
+        forall (P : forall n (dom: t (Sort Var) n) (S: (Var -> Sort EmptySet)) (args: F_args C' S dom), GeneratedArgs _ dom S args -> Prop),
+          (forall n s (dom : t (Sort Var) n) S arg args
+             (arg_gen : AlgebraicallyGenerated (applySubst S s) arg)
+             (args_gen : GeneratedArgs n dom S args),
+              P (Datatypes.S n) (cons _ s n dom) S (arg, args) (GeneratedArgs_cons n s dom S arg args arg_gen args_gen)) ->
+          P (Datatypes.S n) dom S args args_gen := 
+        fun P cons_case =>
+          match args_gen as args_gen' in GeneratedArgs n' dom' S' args' return
+                (n' = Datatypes.S n) -> P n' dom' S' args' args_gen'
+          with
+          | GeneratedArgs_nil S' =>
+            fun eq => False_ind (P 0 (nil _) S' tt (GeneratedArgs_nil S'))
+                             (@eq_ind_r nat (Datatypes.S n)
+                                        (fun x => match x with | Datatypes.S _ => True | _ => False end)
+                                        I _ eq)
+          | GeneratedArgs_cons n s dom S' arg args arg_gen args_gen =>
+            fun eq => cons_case n s dom S' arg args arg_gen args_gen
+          end (eq_refl (Datatypes.S n)).
+      
+      Definition GeneratedArgs_tl n s dom S args (args_gen: GeneratedArgs (Datatypes.S n) (cons _ s n dom) S args):
+        GeneratedArgs n dom S (snd args) :=
+        GeneratedArgs_caseS n (cons _ s n dom) S args args_gen
+                            (fun n' dom' S' args' =>
+                               match dom' with
+                               | nil _ => fun _ _ => GeneratedArgs n dom S (snd args)
+                               | cons _ s n dom => fun (args': F_args C' S' (cons _ s n dom)) gen_args' => GeneratedArgs n dom S' (snd args')
+                               end args')
+                            (fun n s dom S arg args arg_gen args_gen => args_gen).
+
+      Lemma cannonical_morphism_sound: forall s c, AlgebraicallyGenerated s (canonical_morphism s c).
+      Proof.
+        intros s c.
+        apply (fun r => Fix_F A R _ C
+                           (fun s c => AlgebraicallyGenerated s (canonical_morphism s c))
+                           measure r s c (R_wf (measure s c))).
+        clear s c.
+        intros s c IH.
+        rewrite canonical_morphism_commutes.
+        unfold F_mor.
+        generalize (coAlg_decreasing s c).
+        destruct (coAlg s c) as [ op S WF_S args subsort ].
+        simpl.
+        intro args_dec.
+        apply (FromF s op S WF_S (fmap_args C C' S (domain op) canonical_morphism args) subsort).
+        revert args args_dec.
+        generalize (domain op).
+        generalize (arity op).
+        intros n dom.
+        induction dom as [ | s' n dom IH' ].
+        - intros args agrs_dec.
+          simpl.
+          destruct args.
+          apply GeneratedArgs_nil.
+        - intros args args_dec.
+          destruct args as [ arg args ].
+          apply GeneratedArgs_cons.
+          + apply IH.
+            exact (proj1 args_dec).
+          + exact (IH' args (proj2 args_dec)).
+      Qed.
+      
+      Lemma canonical_morphism_complete:
+        forall s c (C_eq_sym: forall s s' c c', C_eq s s' c c' -> C_eq s' s c' c),
+          AlgebraicallyGenerated s c ->
+          exists c', C'_eq s s c (canonical_morphism s c').
+      Proof.
+        intros s c C_eq_sym c_gen.
+        induction c_gen as [ s op S WF_S args subsort args_gen IH ] using AlgebraicallyGenerated_ind'.
+        assert (f_complete: exists f, F_eq C' C'_eq s s (mkF C' s op S WF_S args subsort) (F_mor C C' canonical_morphism s f)).
+        { unfold F_eq.
+          unfold F_mor.
+          simpl.
+          assert (f_args: exists f_args, forall k, C'_eq (applySubst S (nth (domain op) k))
+                                               (applySubst S (nth (domain op) k))
+                                               (F_args_nth C' S (domain op) args k)
+                                               (canonical_morphism (applySubst S (nth (domain op) k))
+                                                                   (F_args_nth C S (domain op) f_args k))).
+          { revert args args_gen IH.
+            generalize (domain op).
+            generalize (arity op).
+            intros n dom args args_gen IH.
+            induction dom as [ | s' n dom IH' ].
+            - exists tt; apply (Fin.case0).
+            - destruct args as [ arg args ].
+              destruct (IH (Fin.F1)) as [ f_arg1 f_arg1_prf ].
+              destruct (IH' args (GeneratedArgs_tl _ _ _ _ _ args_gen) (fun k => IH (Fin.FS k))) as [ f_args f_args_prfs ].
+              exists (f_arg1, f_args).
+              intro k.
+              apply (Fin.caseS' k); assumption. }
+          destruct f_args as [ f_args f_args_prf ].
+          exists (mkF C s op S WF_S f_args subsort).
+          split.
+          - reflexivity.
+          - clear args_gen IH.
+            revert args f_args f_args_prf.
+            simpl.
+            generalize (domain op).
+            generalize (arity op).
+            intros n dom.
+            induction dom as [ | s' n dom IH ].
+            + intros; trivial.
+            + intros args f_args f_args_prf.
+              split.
+              * exact (f_args_prf (Fin.F1)).
+              * exact (IH (snd args) (snd f_args) (fun k => f_args_prf (Fin.FS k))). }
+        destruct f_complete as [ f f_prf ].
+        exists (alg' s f).
+        rewrite canonical_morphism_commutes.
+        apply alg_compat.
+        eapply (F_eq_trans _ C'_eq C'_eq_trans s s s _ _ _ f_prf).
+        apply (F_mor_eq _ _ canonical_morphism C_eq C'_eq canonical_morphism_C_eq_compat).
+        apply (F_eq_sym _ C_eq C_eq_sym).
+        apply (coAlg_alg_inv).
+      Qed.      
     End HomomorphismModulo.
     
   End AlgebraFixpoint.
 
+  Lemma initial_coalg_nth_arg_decreasing:
+    forall s c n,
+      FixF_size _ (F_args_nth FixF (subst _ _ (FixF_coalg s c)) _ (args _ _ (FixF_coalg s c)) n) <
+      FixF_size s c.
+  Proof.
+    intros s c.
+    destruct c as [ op subst subst_wf args subsort ].
+    revert args.
+    simpl.
+    generalize (domain op).
+    generalize (arity op).
+    intros arity argSorts args.
+    induction args as [ | s S arity argSort argSorts arg args IH ]; intro n.
+    - inversion n.
+    - apply (Fin.caseS' n).
+      + simpl.
+        unfold "_ < _".
+        rewrite <- Nat.succ_le_mono.
+        apply Nat.le_add_r.
+      + intro n'.
+        simpl.
+        etransitivity; [ eapply IH; assumption | ].
+        rewrite <- Nat.succ_lt_mono.
+        apply Nat.lt_add_pos_l.
+        unfold FixF_size.
+        destruct arg.
+        unfold "_ < _".
+        apply Nat.le_add_r.
+  Qed.       
     
+  
+  Lemma initial_coalg_decreasing:
+      forall s (c: FixF s),
+        argsDec FixF nat lt FixF_size s c
+                (subst _ _ (FixF_coalg s c)) (domain (op _ _ (FixF_coalg s c))) (args _ _ (FixF_coalg s c)).
+  Proof.
+    intros s c.
+    generalize (initial_coalg_nth_arg_decreasing s c).
+    destruct (FixF_coalg s c) as [ op subst subst_wf args subsort ].
+    simpl.
+    revert args.
+    generalize (domain op).
+    generalize (arity op).
+    intros arity dom.
+    induction dom as [ | argSort n argSorts IH ];
+      intros args dec_prf.
+    - simpl; trivial.
+    - split.
+      + exact (dec_prf Fin.F1).
+      + apply IH.
+        exact (fun k => dec_prf (Fin.FS k)).
+  Qed.      
+  
+  Definition initial_algebra_morphism (C: Sort EmptySet -> Type) (alg: SigmaAlgebra C): forall s, FixF s -> C s :=
+    canonical_morphism FixF C FixF_coalg alg
+                       nat _ (well_founded_ltof _ (fun x => x))
+                       FixF_size initial_coalg_decreasing.
+
+  Definition FixF_args_hd s S n argSort argSorts (args: FixF_args s S _ (cons _ argSort n argSorts)):
+    FixF (applySubst S argSort) :=
+    match args in FixF_args _ S' n' argSorts' return
+          (n' = Datatypes.S n) ->
+          match argSorts' with
+          | nil _ => FixF (applySubst S argSort)
+          | cons _ argSort _ _ => FixF (applySubst S' argSort)
+          end with
+    | FixF_args_nil _ _ =>
+      fun eq =>
+        False_rect _ (@eq_rect_r nat (Datatypes.S n)
+                                 (fun x => match x with | Datatypes.S _ => True | _ => False end)
+                                 I _ eq)
+    | FixF_args_cons _ _ _ _ _ hd _ => fun eq => hd
+    end eq_refl.
+
+  Definition FixF_args_tl s S n argSort argSorts (args: FixF_args s S _ (cons _ argSort n argSorts)):
+    FixF_args s S n argSorts :=
+    match args in FixF_args _ S' n' argSorts' return
+          (n' = Datatypes.S n) ->
+          match argSorts' with
+          | nil _ => FixF_args s S n argSorts
+          | cons _ _ _ argSorts' => FixF_args s S' _ argSorts'
+          end with
+    | FixF_args_nil _ _ =>
+      fun eq =>
+        False_rect _ (@eq_rect_r nat (Datatypes.S n)
+                                 (fun x => match x with | Datatypes.S _ => True | _ => False end)
+                                 I _ eq)
+    | FixF_args_cons _ _ _ _ _ _ tl => fun eq => tl
+    end eq_refl.
+
+  Fixpoint FixF_eq s s' (c: FixF s) {struct c}: FixF s' -> Prop :=
+    fun c' =>
+      match c with
+      | mkFixF _ op subst wf_subst args subsort =>
+        match c' with
+        | mkFixF _ op' subst' wf_subst' args' subsort' =>
+          (op = op') /\
+          ((fix compare_args S S' n (dom1: t (Sort Var) n) m (dom2: t (Sort Var) m) 
+              (args1: FixF_args s S n dom1) (args2: FixF_args s' S' m dom2) {struct args1}: Prop :=
+              match args1 with
+              | FixF_args_cons _ _ _ _ _ hd1 tl1 =>
+                match args2 with
+                | FixF_args_cons _ _ _ _ _ hd2 tl2 =>
+                  (FixF_eq _ _ hd1 hd2) /\ (compare_args _ _ _ _ _ _ tl1 tl2)
+                | _ => False
+                end
+              | FixF_args_nil _ _ =>
+                match args2 with
+                | FixF_args_nil _ _ => True
+                | _ => False
+                end
+              end
+           ) subst subst' _ (domain op) _ (domain op') args args')
+        end
+      end.
+
+  Lemma FixF_eq_refl: forall s (c: FixF s), FixF_eq s s c c.
+  Proof.
+    intros s c.
+    apply (fun r => DepFix nat lt (well_founded_ltof _ (fun x => x)) (Sort EmptySet) FixF (fun s c => FixF_eq s s c c)
+                        (FixF_size) r s c).
+    clear s c.
+    intros s c IH.
+    destruct c as [ op subst wf_subst args subsort ].
+    simpl in IH.
+    split; [ reflexivity | ].
+    revert args IH.
+    generalize (domain op).
+    generalize (arity op).
+    intros arity dom args.
+    induction args as [ | s S n argSort argSorts hd tl IH' ].
+    - intros; trivial.
+    - intro IH.
+      split.
+      + apply IH.
+        unfold "_ < _".
+        rewrite <- Nat.succ_le_mono.
+        apply Nat.le_add_r.
+      + apply IH'; try solve [ assumption ].
+        intros s' arg arg_dec.
+        apply IH.
+        rewrite (Nat.add_comm 1).
+        rewrite <- (Nat.add_assoc).
+        rewrite (Nat.add_comm _ 1).
+        etransitivity; [ apply arg_dec | ].
+        apply Nat.lt_add_pos_l.
+        destruct hd.
+        simpl.
+        unfold "_ < _".
+        apply Nat.le_add_r.
+  Qed.
+
+  Lemma FixF_eq_trans: forall s1 s2 s3 c1 c2 c3,
+      FixF_eq s1 s2 c1 c2 -> FixF_eq s2 s3 c2 c3 -> FixF_eq s1 s3 c1 c3.
+  Proof.
+    intros s1 s2 s3 c1 c2.
+    revert s1 s3 c1.
+    apply (fun r => DepFix nat lt (well_founded_ltof _ (fun x => x)) (Sort EmptySet) FixF
+                        (fun s2 c2 => forall s1 s3 c1 c3, FixF_eq s1 s2 c1 c2 -> FixF_eq s2 s3 c2 c3 -> FixF_eq s1 s3 c1 c3)
+                        (FixF_size) r s2 c2).
+    clear s2 c2.
+    intros s2 c2 IH s1 s3 c1 c3.
+    unfold FixF_eq.
+    destruct c1 as [ op1 subst1 wf_subst1 args1 subsort1 ].
+    destruct c2 as [ op2 subst2 wf_subst2 args2 subsort2 ].
+    destruct c3 as [ op3 subst3 wf_subst3 args3 subsort3 ].
+    intros [ op12 args12 ] [ op23 args23 ].
+    split.
+    - etransitivity; [ exact op12 | exact op23 ].
+    - revert IH.
+      simpl.
+      revert args1 args3 args12 args23.
+      assert (arity_eq12 : arity op1 = arity op2).
+      { rewrite op12; reflexivity. }
+      assert (arity_eq32 : arity op3 = arity op2).
+      { rewrite <- op23; reflexivity. }
+      assert (domain_eq12 : rew arity_eq12 in domain op1 = domain op2).
+      { revert arity_eq12.
+        rewrite op12.
+        intro arity_eq12.
+        rewrite (UIP_dec Nat.eq_dec arity_eq12 eq_refl).
+        reflexivity. }
+      assert (domain_eq32: rew arity_eq32 in domain op3 = domain op2).
+      { revert arity_eq32.
+        rewrite <- op23.
+        intro arity_eq32.
+        rewrite (UIP_dec Nat.eq_dec arity_eq32 eq_refl).
+        reflexivity. }
+      revert args2 arity_eq12 arity_eq32 domain_eq12 domain_eq32.
+      generalize (domain op2).
+      generalize (arity op2).
+      intros arity2 argSorts2 args2.
+      generalize (domain op1).
+      generalize (arity op1).
+      generalize (domain op3).
+      generalize (arity op3).        
+      induction args2 as [ | s2 S2 n2 argSort2 argSorts2 arg2 args2 IH' ].
+      + intros arity3 dom3 arity1 dom1.
+        destruct arity1; intro arity_eq12; [ | inversion arity_eq12 ].
+        destruct arity3; intro arity_eq32; [ | inversion arity_eq32 ].
+        rewrite (UIP_dec Nat.eq_dec arity_eq12 eq_refl).
+        rewrite (UIP_dec Nat.eq_dec arity_eq32 eq_refl).
+        simpl.
+        intros dom1_eq dom3_eq.
+        rewrite dom1_eq.
+        rewrite dom3_eq.
+        intros args1 args3.
+        apply (fun P r => FixF_args_case0 s1 subst1 P (nil _) args1 r).
+        intro.
+        destruct args3.
+        * intros; trivial.
+        * intro; contradiction.
+      + intros arity3 dom3 arity1 dom1.
+        destruct arity1; intro arity_eq12; [ inversion arity_eq12 | ].
+        inversion arity_eq12 as [ arity_eq12' ].
+        revert dom1 arity_eq12; rewrite arity_eq12'.
+        intros dom1 arity_eq12.
+        rewrite (UIP_dec Nat.eq_dec arity_eq12 eq_refl).
+        clear arity_eq12.
+        simpl.
+        intros arity_eq32 dom1_eq dom3_eq args1 args3.
+        revert dom1_eq arity_eq32 dom3_eq IH'.
+        apply (FixF_args_caseS' s1 subst1 _ _ args1).
+        clear args1 wf_subst1 subsort1 subst1.
+        intros subst1 argSort1 argSorts1 arg1 args1 dom1_eq.
+        destruct args3 as [ | subst3 arity3 argSort3 argSorts3 arg3 args3 ].
+        * intros; contradiction.
+        * inversion arity_eq32 as [ arity_eq32' ].
+          revert argSorts3 arity_eq32 args3; rewrite arity_eq32'.
+          intros argSorts3 arity_eq32 args3.
+          rewrite (UIP_dec Nat.eq_dec arity_eq32 eq_refl).
+          clear arity_eq32.
+          simpl.
+          intros dom3_eq IH' [ arg12 args12 ] [ arg23 args23 ] IH.
+          split.
+          { apply (IH _ arg2); try solve [ assumption ].
+            unfold "_ < _".
+            rewrite <- Nat.succ_le_mono.
+            apply Nat.le_add_r. }
+          { apply (IH' wf_subst2 subsort2 _ _ _ _ eq_refl eq_refl); try solve [ assumption ].
+            - simpl.
+              inversion dom1_eq as [ [ argSort12_eq argSorts12_eq ] ].
+              exact (vect_exist_eq _ _ argSorts12_eq).
+            - simpl.
+              inversion dom3_eq as [ [ argSort32_eq argSorts32_eq ] ].
+              exact (vect_exist_eq _ _ argSorts32_eq).
+            - intros s arg arg_dec.
+              apply IH.
+              rewrite (Nat.add_comm 1).
+              rewrite <- (Nat.add_assoc _ _ 1).
+              rewrite (Nat.add_comm _ 1).
+              etransitivity; [ exact arg_dec | ].
+              apply Nat.lt_add_pos_l.
+              destruct arg2.
+              unfold FixF_size.
+              simpl.
+              unfold "_ < _".
+              apply Nat.le_add_r. }
+  Qed.
+        
+  Lemma FixF_eq_sym: forall s s' (c: FixF s) (c': FixF s'), FixF_eq s s' c c' -> FixF_eq s' s c' c.
+  Proof.
+    intros s s' c.
+    revert s'.
+    apply (fun r => DepFix nat lt (well_founded_ltof _ (fun x => x)) (Sort EmptySet) FixF
+                        (fun s c => forall s' c', FixF_eq s s' c c' -> FixF_eq s' s c' c)
+                        (FixF_size) r s c).
+    clear s c.
+    intros s c IH s' c'.
+    destruct c as [ op subst wf_subst args subsort ].
+    destruct c' as [ op' subst' wf_subst' args' subsort' ].
+    intros [ op_eq args_eq ].
+    split; [ rewrite op_eq; reflexivity | ].
+    revert args' args_eq.
+    assert (arity_eq: arity op' = arity op).
+    { rewrite op_eq; reflexivity. }
+    assert (dom_eq: rew arity_eq in domain op' = domain op).
+    { revert arity_eq.
+      rewrite <- op_eq.
+      intro arity_eq.
+      rewrite (UIP_dec Nat.eq_dec arity_eq eq_refl).
+      reflexivity. }
+    revert args IH arity_eq dom_eq.      
+    simpl.
+    generalize (domain op).
+    generalize (arity op).
+    intros arity1 dom args.
+    generalize (domain op').
+    generalize (arity op').
+    induction args as [ | s subst arity1 argSort argSorts arg args IH' ].
+    - intros arity2 dom2 IH.
+      destruct arity2; intro arity_eq; [ | inversion arity_eq ].
+      rewrite (UIP_dec Nat.eq_dec arity_eq eq_refl).
+      simpl.
+      intro dom2_eq.
+      intro args'.
+      apply (fun P r => FixF_args_case0 s' subst' P dom2 args' r).
+      intro; trivial.
+    - intros arity2 dom2 IH.
+      destruct arity2; intro arity_eq; [ inversion arity_eq | ].
+      inversion arity_eq as [ arity_eq' ].
+      revert arity_eq dom2.
+      rewrite arity_eq'.
+      intros arity_eq dom2.
+      rewrite (UIP_dec Nat.eq_dec arity_eq eq_refl).
+      simpl.
+      intros dom_eq args2.
+      clear arity_eq.
+      revert dom_eq IH'.
+      apply (FixF_args_caseS' s' subst' _ _ args2).
+      clear args2 subst' dom2 wf_subst' subsort'.
+      intros subst' argSort' argSorts' arg' args' argSorts_eq IH' [ arg_eq args_eq ].
+      split.
+      + apply IH; [ | assumption ].
+        unfold "_ < _".
+        rewrite <- Nat.succ_le_mono.
+        apply Nat.le_add_r.
+      + apply (fun rec eq => IH' wf_subst subsort _ _ rec eq_refl eq _ args_eq).
+        * intros s'' arg'' arg''_dec.
+          apply IH.
+          rewrite arg''_dec.
+          rewrite <- (Nat.succ_lt_mono).
+          apply Nat.lt_add_pos_l.
+          unfold FixF_size.
+          destruct arg.
+          unfold "_ < _".
+          apply Nat.le_add_r.
+        * inversion argSorts_eq as [ [ argSort_eq argSorts_eq' ] ].
+          simpl.
+          exact (vect_exist_eq _ _ argSorts_eq').
+  Qed.
+
+  Section StrongUniqueness.
+    Variable Carrier': Sort EmptySet -> Type.
+    Variable algebra: SigmaAlgebra Carrier'.
+    
+    Definition unique_mor := initial_algebra_morphism Carrier' algebra.
+
+    Lemma initial_morphism_alg_mor:
+      forall s f,
+         (unique_mor s (FixF_alg s f)) =
+         (algebra s (F_mor FixF Carrier' unique_mor s f)).
+    Proof.
+      intros s f.
+      unfold unique_mor.
+      unfold initial_algebra_morphism.
+      rewrite canonical_morphism_commutes.
+      rewrite FixF_alg_coalg.
+      reflexivity.
+    Qed.
+
+    Lemma fmap_args_dec_fmap_args_eq
+     : forall (C C' : Sort EmptySet -> Type) (A : Type) (R : A -> A -> Prop)
+         (measure : forall s : Sort EmptySet, C s -> A) (S : Var -> Sort EmptySet) (n : nat)
+         (params : t (Sort Var) n) (s : Sort EmptySet) (c : C s)
+         (f: forall (s' : Sort EmptySet) (c' : C s'), R (measure s' c') (measure s c) -> C' s')
+         (g: forall (s' : Sort EmptySet), C s' -> C' s')
+         (args : F_args C S params) (args_dec: argsDec C A R measure s c S params args),
+        (forall s' c' (acc: R (measure s' c') (measure s c)), f s' c' acc = g s' c') ->
+        fmap_args_dec C C' A R measure S params s c f args args_dec =
+        fmap_args C C' _ params g args.
+    Proof.
+      intros C C' A R measure S n params s c f g args args_dec eqprf.
+      revert args args_dec.
+      induction params as [ | param n params IH ].
+      - intros args args_dec.
+        destruct args.
+        reflexivity.
+      - intros args args_dec.
+        simpl.
+        rewrite eqprf.
+        rewrite IH.
+        reflexivity.
+    Qed.
+
+    Lemma initial_morphism_unique:
+      forall (g: forall s, FixF s -> Carrier' s),
+        (forall s f, g s (FixF_alg s f) = algebra s (F_mor FixF Carrier' g s f)) ->
+        forall s c, g s c = unique_mor s c.
+    Proof.
+      intros g g_alg_mor s c.
+      unfold unique_mor.
+      unfold initial_algebra_morphism.
+      unfold canonical_morphism.
+      unfold DepFix.
+      generalize (well_founded_ltof nat (fun x => x) (FixF_size s c)).
+      match goal with
+      |[|- forall acc, g s c = (?f_rec s c acc)] =>
+       apply (fun r => Fix_F nat (ltof nat (fun x => x)) (Sort EmptySet) FixF
+                          (fun s c => forall acc, g s c = f_rec s c acc) FixF_size
+                          r s c (well_founded_ltof nat (fun x => x) (FixF_size s c)))
+      end.
+      clear s c.
+      intros s c IH acc.
+      rewrite <- (FixF_coalg_alg s c) at 1.
+      rewrite g_alg_mor.
+      destruct acc as [ acc' ].
+      simpl.
+      unfold F_mor.
+      destruct c as [ op subst wf_subst args subsort ].
+      simpl.
+      apply (f_equal (fun args' =>
+                        algebra s {| op := op; subst := subst;
+                                     wf_subst := wf_subst; args := args';
+                                     subsort := subsort |})).
+      apply eq_sym.
+      apply (fmap_args_dec_fmap_args_eq).
+      intros s' c' acc.
+      apply eq_sym.
+      eapply IH.
+      exact acc.
+    Qed.
+  End StrongUniqueness.
+      
+  
+    (*Section UniquenessModulo.
+      Lemma initial_morphism_alg_mor:
+        forall s s' f f',
+          F_eq FixF (fun s s' => s = s') s s' f f' ->
+          carrier'_eq s s' (unique_mor s (FixF_alg s f))
+                      (algebra s' (F_mor FixF Carrier' unique_mor s' f')).
+      Proof.
+        apply canonical_morphism_alg_mor; try solve [ assumption ].
+        - exact carrier_eq_trans.
+        - exact (F_eq_compat_coalg CL_dec).
+        - intros.
+          apply F_eq_sym; [ exact carrier_eq_sym | ].
+          apply (CL_AlgebraCoAlgebra_inv CL_dec).
+      Qed.
+
+      Lemma CL_Algebra_morphism_unique:
+        forall (morphism: forall s, Carrier s -> Carrier' s)
+          (morphism_compat:
+             forall s s' c c', carrier_eq s s' c c' -> carrier'_eq s s' (morphism s c) (morphism s' c'))
+          (morphism_alg_homo:
+             forall s s' f f',
+               F_eq Carrier carrier_eq s s' f f' ->
+               carrier'_eq s s' (morphism s (CL_Algebra s f)) (algebra s' (F_mor Carrier Carrier' morphism s' f')))
+          s c,
+          carrier'_eq s s (morphism s c) (unique_mor s c).
+      Proof.
+        apply canonical_morphism_unique.
+        - exact carrier_eq_refl.
+        - exact carrier'_eq_trans.
+        - exact alg_compat.
+        - intros s c.
+          apply carrier_eq_sym.
+          exact (CL_CoAlgebraAlgebra_inv CL_dec s c).
+      Qed.
+    End UniquenessModulo. *)
 End Algebraic.
 
